Compiler/Skeletons/mkMap.v
@@ -1,14 +1,15 @@
 Require Import LibTactics Psatz.
 Require Import GPUCSL SkelLib scan_lib CSLTactics.
 Require Import CUDALib TypedTerm.
-Require Import Skel_lemma CSLLemma CodeGen CUDALib Correctness CSLTactics.
 Require Import Host.
-
-Open Scope string_scope.
+Require Import Skel_lemma CodeGen CUDALib Correctness Grid CSLTactics CSLLemma.
 
 Section mkMap.
 
 Variable ntrd nblk : nat.
+
+Hypothesis ntrd_neq_0: ntrd <> 0.
+Hypothesis nblk_neq_0: nblk <> 0.
 
 Variable GA : list Skel.Typ.
 Variable avar_env : AVarEnv GA.
@@ -28,7 +29,6 @@ Hypothesis f_ok : func_ok avar_env f f_c.
 Variable result : Skel.aTypDenote cod.
 Hypothesis eval_map_ok :
   Skel.skelDenote _ _ (Skel.Map _ _ _ f arr) aeval_env = Some result.
-
 Lemma eval_arr_ok :
   { arr_res | Skel.aeDenote _ _ arr aeval_env = Some arr_res}.
 Proof.
@@ -42,6 +42,8 @@ Definition eval_arr_ok' : Skel.aeDenote _ _ arr aeval_env = Some arr_res.
 Proof.
   unfold arr_res; destruct eval_arr_ok; eauto.
 Qed.
+
+Hint Resolve eval_arr_ok' : pure_lemma.
 
 Lemma eval_f_ok : 
   { f_res | forall i, i < length arr_res ->
@@ -66,26 +68,27 @@ Definition outArr ty := locals "_arrOut" ty 0.
 
 Notation out := (outArr cod).
 Notation len := out_len_name.
-Definition t := locals "t" dom 0.
+Notation t := (locals "t" dom 0).
 
 Definition mkMap_cmd inv :=
   "i" :T Int ::= "tid" +C "bid" *C Zn ntrd ;;
   WhileI inv ("i" <C len) (
-    fst (arr_c "i") ;;
-    assigns t (ty2ctys dom) (v2e (snd (arr_c "i"))) ;;
+    assigns_get t arr_c "i" ;;
     fst (f_c t) ;;
     writes (v2gl out +os "i") (v2e (snd (f_c t))) ;;
     "i" ::= Zn ntrd *C Zn nblk +C "i"
   )%exp.
+
+Definition mkMap_prog :=
+  Pr nil (mkMap_cmd FalseP).
 
 Definition mkMap : kernel :=
   let arr_vars := gen_params GA in
   let params_in := flatten_avars arr_vars in
   let params_out := (out_len_name, Int) :: flatTup (out_name cod) in
   {| params_of := params_out ++ params_in;
-     body_of := GCSL.Pr nil (mkMap_cmd FalseP) |}.
+     body_of := mkMap_prog |}.
 
-Notation RP n := (1 / injZ (Zn n))%Qc.
 Notation p := (RP (nblk * ntrd)).
 
 Variable outp : vals cod.
@@ -94,62 +97,307 @@ Hypothesis outs_length : length outs = length result.
 Definition outRes (ls : list (vals cod)) := arrays (val2gl outp) ls 1.
 Definition outEnv := out |=> outp.
 
+Notation result' := (arr2CUDA result).
+
 Section thread_ok.
 Variable tid : Fin.t ntrd.
 Variable bid : Fin.t nblk.
 
+
+Lemma tid_bid : nf tid + nf bid * ntrd < ntrd * nblk.
+Proof.
+  pose proof ntrd_neq_0; pose proof nblk_neq_0.
+  assert (nf tid < ntrd) by eauto.
+  assert (nf bid < nblk) by eauto.
+  forwards*: (id_lt_nt_gr H1 H2).
+  lia.
+Qed.
+
 Notation arri a := (skip a (ntrd * nblk) (nf tid + nf bid * ntrd)).
-Notation result' := (arr2CUDA result).
 
 Definition inv'  :=
   Ex j i,
   (kernelInv avar_env aptr_env aeval_env 
              (arrays' (val2gl outp) (arri (firstn i result' ++ skipn i outs)) 1) 
-             (i = j * (ntrd * nblk) + (nf tid + nf bid * nblk) /\
-              i < length arr_res)
+             (i = j * (ntrd * nblk) + (nf tid + nf bid * ntrd) /\
+              i < length arr_res + ntrd * nblk)
              (len |-> Zn (length arr_res) ::
               "i" |-> Zn i ::
               out |=> outp) p).
 
-Ltac prove_not_local :=
-  let x := fresh "x" in
-  let H := fresh "H" in
-  simpl; intros x H;
-  des_disj H; substs;
-  unfold is_param; simpl; try congruence.
+Ltac t :=
+  autorewrite with pure; simpl;
+  abstract (repeat match goal with
+                   | [|- context [if ?b then _ else _]] => destruct b; substs; eauto; try (false; lia); try lia
+                   | [H : context [if ?b then _ else _] |- _] => destruct b; substs; eauto; try (false; lia); try lia
+                   end;
+             do 2 f_equal; lia). 
 
-Lemma remove_var_out ty ps x :
-  prefix "_" x = false
-  -> remove_var (outArr ty |=> ps) x = outArr ty |=> ps.
+
+Lemma ok1 n m j : n + (j * n + m) = (S j) * n + m. nia. Qed.
+Lemma ok2 n m : m = 0 * n + m. nia. Qed.
+Lemma ntrd_nblk_neq_0 : ntrd * nblk <> 0. pose ntrd_neq_0; pose nblk_neq_0; nia. Qed.
+
+Hint Resolve ok1 ok2 tid_bid ntrd_nblk_neq_0 : pure_lemma.
+
+Lemma loop_inv_ok i j vs (varr vout : list (vals cod)) v:
+  i = j * (ntrd * nblk) + (nf tid + nf bid * ntrd) ->
+  vs = firstn i varr ++ skipn i vout ->
+  (Zn i < Zn (length varr))%Z ->
+  length varr = length vout ->
+  v = gets varr i ->
+  arri (set_nth i vs v) =
+  arri (firstn (ntrd * nblk + i) varr ++ skipn (ntrd * nblk + i) vout).
 Proof.
-  intros Hpref.
-  apply remove_var_disjoint; simpl.
-  unfold outArr; intros Hc.
-  apply in_map_iff in Hc as (? & ? & ?); substs.
-  destruct x0; simpl in *.
-  apply mpss_in in H0.
-  forwards* (j & Heq & ?): locals_pref; substs.
-  inverts Heq; simpl in *; congruence.
+  intros; substs.
+  applys (>>(@eq_from_nth) (@None (vals cod))).
+  { t. }
+  { intros i; repeat autorewrite with pure; simpl in *.
+    destruct lt_dec; [|false; lia]; intros H.
+    assert (i = j * (ntrd * nblk) + (nf tid + nf bid * ntrd) ->
+            i mod (ntrd * nblk) = nf tid + nf bid * ntrd) by (intros; substs; prove_mod_eq).
+    assert (ntrd * nblk <> 0) by eauto with pure_lemma.
+    assert (j * (ntrd * nblk) + (nf tid + nf bid * ntrd) < i < S j * (ntrd * nblk) + (nf tid + nf bid * ntrd) ->
+            i mod (ntrd * nblk) <> nf tid + nf bid * ntrd).
+    { intros; apply (mod_between j); eauto with pure_lemma. }
+    
+    Time t. }
+Qed.
+
+Lemma before_loop_ok (varr vout : list (vals cod)) :
+  nf tid < ntrd ->
+  nf tid + nf bid * ntrd < ntrd * nblk ->
+  length varr = length vout ->
+  arri vout =
+  arri (firstn (nf tid + nf bid * ntrd) varr ++ skipn (nf tid + nf bid * ntrd) vout).
+Proof.
+  intros; applys (>>(@eq_from_nth) (@None (vals cod))).
+  { t. }
+  { intros.
+    repeat autorewrite with pure; simpl in *.
+    assert (i < nf tid + nf bid * ntrd -> (i mod (ntrd * nblk)) <> nf tid + nf bid * ntrd).
+    { intros; rewrite Nat.mod_small; eauto; try lia. }
+  Time t. }
+Qed.
+
+Lemma after_loop_ok (varr vout : list (vals cod)) vs i :
+  ~(Zn i < Zn (length varr))%Z ->
+  length varr = length vout ->
+  vs = firstn i varr ++ skipn i vout ->
+  arri vs = arri varr.
+Proof.
+  intros; substs; eapply (@eq_from_nth _ None).
+  { t. }
+  intros i'; repeat autorewrite with pure; simpl; intros ?.
+  Time t.
+Qed.
+
+Hint Resolve loop_inv_ok before_loop_ok after_loop_ok : pure_lemma.
+
+Lemma result_nth i :
+  i < length result -> gets' result i = f_res i.
+Proof.
+  simpl in *; unfold Monad.bind_opt in *.
+  generalize arr_res eval_f_ok'  eval_arr_ok' eval_map_ok; intros arr_res' ? Heq.
+  rewrite Heq; intros.
+  forwards*: (>>mapM_some i (@defval' dom)).
+  forwards*: mapM_length; eauto.
+  destruct lt_dec; try lia.
+  rewrite H in H1; eauto.
+  inverts H1.
+  eauto.
 Qed.
 
 Lemma mkMap_cmd_ok BS : 
   CSL BS tid
-      (kernelInv avar_env aptr_env aeval_env (arrays' (val2gl outp) (arri outs) 1)
-                 True
-                 ("tid" |-> Zn (nf tid)
-                  :: "bid" |-> Zn (nf bid)
-                  :: len |-> Zn (length arr_res)
-                  :: out |=> outp) p)
+      (kernelInv
+         avar_env aptr_env aeval_env
+         (arrays' (val2gl outp) (arri outs) 1)
+         True
+         ("tid" |-> Zn (nf tid) ::
+          "bid" |-> Zn (nf bid) ::
+          len |-> Zn (length arr_res) ::
+          out |=> outp) p)
       (mkMap_cmd inv')
-      (kernelInv avar_env aptr_env aeval_env (arrays' (val2gl outp) (arri (arr2CUDA result)) 1) True nil p).
+      (kernelInv'
+         aptr_env aeval_env
+         (arrays' (val2gl outp) (arri (arr2CUDA result)) 1)
+         True p).
 Proof.
+  assert (Hlen: length arr_res = length result').
+  { generalize arr_res eval_arr_ok' eval_map_ok; simpl in *; unfold Monad.bind_opt in *; intros a Heq.
+    rewrite Heq; intros H.
+    forwards*: mapM_length; eauto.
+    unfold arr2CUDA; rewrite map_length; eauto. }
+  assert (Hlen' : length outs = length result').
+  { unfold arr2CUDA; rewrite map_length; eauto. }
+  forwards*: (nf_lt tid).
+  forwards*: (tid_bid).
   eapply rule_seq.
-  applys* kernelInv_inner.
-  prove_not_local. 
+  hoare_forward_prim'; simplify_remove_var.
+  unfold inv'.
+
+  hoare_forward; simplify_remove_var.
+  hoare_forward; simplify_remove_var.
+  hoare_forward; simplify_remove_var.
+  intros; apply eval_f_ok'; lia.
+  assert (ntrd * nblk <> 0) by nia.
   hoare_forward.
-  rewrite remove_var_out; eauto.
-  unfold inv'; hoare_forward.
-  hoare_forward.
-Abort.
+  hoare_forward; simplify_remove_var.
+
+  unfold kernelInv; prove_imp.
+  eapply loop_inv_ok; eauto; prove_pure.
+  unfold arr2CUDA; rewrites (>>nth_map (@defval cod)); prove_pure.
+  rewrite result_nth; eauto; lia.
+  prove_imp; eauto with pure_lemma.
+  unfold kernelInv; simpl in *.
+  prove_imp; eauto with pure_lemma; try tauto.
+  eapply after_loop_ok; [..|eauto]; prove_pure.
+Qed.
 End thread_ok.
+
+Section block_ok.
+Variable bid : Fin.t nblk.
+
+Notation fin_star n f :=
+  (istar (ls_init 0 n f)).
+
+Definition ith_pre (tid : Fin.t ntrd) :=
+  (kernelInv
+     avar_env aptr_env aeval_env
+     (arrays' (val2gl outp) (skip outs (ntrd * nblk) (nf tid + nf bid * ntrd)) 1)
+     True
+     ("bid" |-> Zn (nf bid) ::
+      len |-> Zn (length arr_res) ::
+      out |=> outp) p).
+
+Definition ith_post (tid : Fin.t ntrd) :=
+  (kernelInv'
+     aptr_env aeval_env
+     (arrays' (val2gl outp) (skip (arr2CUDA result) (ntrd * nblk) (nf tid + nf bid * ntrd)) 1)
+     True
+     p).
+
+Definition jth_pre : assn :=
+  kernelInv
+    avar_env aptr_env aeval_env 
+    (fin_star ntrd (fun i => arrays' (val2gl outp) (skip outs (ntrd * nblk) (i + (nf bid) * ntrd)) 1))
+    True
+    (len |-> Zn (length arr_res) ::
+     out |=> outp) (p * injZ (Zn ntrd)).
+
+Definition jth_post : assn :=
+  kernelInv'
+    aptr_env aeval_env 
+    (fin_star ntrd (fun i => arrays' (val2gl outp) (skip result' (ntrd * nblk) (i + (nf bid) * ntrd)) 1))
+    True (p * injZ (Zn ntrd)).
+
+Definition E := fun x : var =>
+  if prefix "_" (str_of_var x) then Lo
+  else if var_eq_dec "bid" x then Lo
+  else Hi.
+
+Definition BS (n : nat) := default ntrd.
+
+Lemma mkMap_cmd_ok_b :
+  CSLp ntrd E
+       (jth_pre ** !("bid" === Zn (nf bid)))
+       (mkMap_cmd TrueP)
+       jth_post.
+Proof.
+  unfold jth_pre, jth_post.
+  applys (>>rule_block BS E (MyVector.init ith_pre) (MyVector.init ith_post)); eauto;
+  unfold BS, ith_pre, ith_post.
+  - unfold default; split; intros; simpl; rewrite MyVector.init_spec; prove_low_assn.
+  - unfold default; split; intros; simpl; rewrite MyVector.init_spec; prove_precise.
+  - intros s h; rewrite kernelInv_var_in; revert s h; prove_istar_imp.
+  - prove_istar_imp.
+  - unfold E; introv; rewrite MyVector.init_spec; prove_low_assn.
+  - unfold E; introv; rewrite MyVector.init_spec.
+    apply low_assn_vars; simpl in *; tauto.
+  - unfold E, mkMap_cmd.
+    instantiate (1 := Hi).
+    unfold assigns_get; repeat prove_typing_cmd.
+  - intros; rewrite !MyVector.init_spec.
+    eapply rule_conseq; eauto using mkMap_cmd_ok.
+    unfold kernelInv; introv; rewrite assn_var_in; revert s h; prove_imp.    
+    
+Qed.
+
+End block_ok.    
+
+Require Import QArith.
+Close Scope Q_scope.
+Lemma n_neq_0_Q n :
+  n <> 0 -> ~(inject_Z (Zn n) == 0)%Q.
+Proof.
+  intros.
+  destruct n; try lia.
+  lets: (>>inject_Z_Sn_gt0 n).
+  lra.
+Qed.
+
+Hint Resolve n_neq_0_Q.
+
+Lemma mkMap_prog_ok :
+  CSLg ntrd nblk
+       (kernelInv avar_env aptr_env aeval_env
+                  (arrays (val2gl outp) outs 1)
+                  True
+                  (len |-> Zn (length arr_res) :: out |=> outp) 1)
+       mkMap_prog
+       (kernelInv' aptr_env aeval_env 
+                  (arrays (val2gl outp) result' 1)
+                  True 1).
+Proof.
+  assert (Heq : (p * injZ (Zn ntrd) = 1 / injZ (Zn nblk))%Qc).
+  { unfold injZ; Qc_to_Q.
+    rewrite Nat2Z.inj_mul, inject_Z_mult. 
+    field; eauto. }
+  assert (Heq' : (1 = RP nblk * injZ (Zn nblk))%Qc).
+  { unfold injZ; Qc_to_Q; field; eauto. }    
+  applys* (>> rule_grid E (MyVector.init jth_pre) (MyVector.init jth_post));
+  unfold jth_pre, jth_post; repeat rewrite Heq.
+  - intros s h H; rewrite Heq' in H; revert s h H.
+    prove_istar_imp.
+    simpl_nested_istar.
+    rewrite CodeGen.array'_ok.
+    rewrite <-Heq' in *; eauto.
+    intros; rewrite mult_comm; apply Nat.mod_upper_bound; nia.
+  - unfold kernelInv; introv; rewrite !MyVector.init_spec.
+    apply CSLp_preprocess; simpl.
+    destruct locs; destruct vss; simpl; try lia.
+    unfold sh_spec_assn; simpl.
+    intros _ _; eapply rule_p_backward; [|intros; rewrite Assn_combine in *; eauto].
+    apply rule_p_assn; intros.
+    eapply rule_p_conseq; try applys (>>mkMap_cmd_ok_b bid); unfold jth_pre, jth_post, kernelInv.
+    + intros s h Hsat; rewrite assn_var_in; revert s h Hsat; prove_imp.
+      rewrite <-!res_assoc, Heq in *.
+      repeat sep_cancel'.
+    + intros s h Hsat.
+      exists (@nil (list val)); split; simpl; unfold Apure; eauto.
+      fold_sat; unfold sh_spec_assn'.
+      revert s h Hsat; prove_imp; simpl in *; try tauto.
+      rewrite <-!res_assoc, Heq in *; simpl in *.
+      repeat sep_cancel'.
+  - prove_istar_imp.
+    simpl_nested_istar.
+    rewrite <-Heq' in *.
+    rewrite CodeGen.array'_ok  in *; eauto.
+    intros; rewrite mult_comm; apply Nat.mod_upper_bound; nia.
+  - intros; rewrite MyVector.init_spec.
+    apply inde_assn_vars.
+    unfold outArr, len, name_of_len.
+    prove_low_expr; intros Hc; des_disj Hc; eauto; try congruence; substs.
+    forwards* H': mpss_in; forwards* (? & ? & ?): (>>locals_pref H'); substs; inverts H.
+    forwards* H': mpss_in; forwards* (? & ? & ?): (>>locals_pref H'); substs; inverts H.
+    forwards*: aenv_ok_params; simpl in *; congruence.
+    forwards*: aenv_ok_params; simpl in *; congruence.
+  - intros; rewrite MyVector.init_spec.
+    unfold E; prove_low_assn.
+  - intros; rewrite MyVector.init_spec; unfold kernelInv. 
+    apply has_no_vars_assn.
+  - simpl; tauto.
+  - simpl; tauto.
+Qed.
 End mkMap.
